wordarray wip: Working on generic fold corres lemmas

cogent/examples/wa_connect/WordArray_UpdCCorresGen.thy
@@ -5,8 +5,6 @@ theory WordArray_UpdCCorresGen
   imports WordArray_UAbsFun
 begin
 
-
-
 context WordArray begin
 
 section "Helper Lemmas"
@@ -34,23 +32,30 @@ subsection "wordarray_length"
 definition wordarray_length_c
   where
   "wordarray_length_c is_v h l p \<equiv>
-    do _ <- guard (\<lambda>s. is_v s p);
-       ret <- do _ <- guard (\<lambda>s. is_v s p);
-             gets (\<lambda>s. SCAST(32 signed \<rightarrow> 32) (l (h s p)))
-              od;
-       global_exn_var <- gets (\<lambda>_. Return);
-       _ <- gets (\<lambda>_. ());
-       gets (\<lambda>_. ret)
-    od"
+     do _ <- guard (\<lambda>s. is_v s p);
+        ret <- do _ <- guard (\<lambda>s. is_v s p); gets (\<lambda>s. SCAST(32 signed \<rightarrow> 32) (l (h s p))) od;
+        global_exn_var <- gets (\<lambda>_. Return);
+        _ <- gets (\<lambda>_. ());
+        gets (\<lambda>_. ret)
+     od"
 
 lemma upd_C_wordarray_length_c_corres_gen:
   "\<And>i \<gamma> v' \<Gamma>' \<sigma> st.
-    \<lbrakk>\<Xi>' fn = ([], TCon ''WordArray'' [TPrim (Num num)] (Boxed ReadOnly ptrl), TPrim (Num U32));
+    \<lbrakk>\<comment>\<open>The type of wordarray_length, where @{term fn} is name of the wordarray_length function in C,
+        @{term num} is the numeric type of the word array and @{term ptrl} is the pointer layout\<close>
+     \<Xi>' fn = ([], TCon ''WordArray'' [TPrim (Num num)] (Boxed ReadOnly ptrl), TPrim (Num U32));
+     \<comment>\<open>The embedding of wordarray_length in the update semantics\<close>
      \<xi>0' fn = upd_wa_length_0;
+     \<comment>\<open>For all related Cogent and C states, the Cogent and C heaps for word arrays are related\<close>
      \<forall>x y. (x, y) \<in> srel \<longrightarrow> (\<forall>(p :: ('a :: cogent_C_val) ptr) uv. heap_rel_meta is_v h x y p);
+     \<comment>\<open>The type relation for word arrays\<close>
      type_rel (RCon ''WordArray'' [RPrim (Num num)]) TYPE('a);
+     \<comment>\<open>The value relation for word arrays, where @{term l_c} extracts the length value and
+        @{term v_c} extracts the pointer to the array of words\<close>
      \<forall>uv (cv :: 'a). val_rel uv cv = (\<exists>len arr. uv = UAbstract (UWA (TPrim (Num num)) len arr) \<and>
         len = (SCAST(32 signed \<rightarrow> 32)(l_c cv)) \<and> arr = ptr_val (v_c cv));
+     \<comment>\<open>The rest of the assumptions are the standard value relation of arguments and what their
+        types are\<close>
      i < length \<gamma>;
      val_rel (\<gamma> ! i) v';
      \<Gamma>' ! i = option.Some (prod.fst (prod.snd (\<Xi>' fn)))\<rbrakk>
@@ -84,54 +89,110 @@ lemma upd_C_wordarray_length_c_corres_gen:
   apply (erule_tac x = v' in allE)
   apply (clarsimp simp: heap_rel_meta_def type_rel_simp wa_abs_repr_def)
   done
+(*
+lemma upd_C_wordarray_length_c_corres_gen':
+  assumes
+    \<comment>\<open>The type of wordarray_length, where @{term fn} is name of the wordarray_length function in C,
+        @{term num} is the numeric type of the word array and @{term ptrl} is the pointer layout\<close>
+    fntyp: "\<Xi>' fn = ([], TCon ''WordArray'' [TPrim (Num num)] (Boxed ReadOnly ptrl), TPrim (Num U32))"
+  and
+    \<comment>\<open>The embedding of wordarray_length in the update semantics\<close>
+    embed: "\<xi>0' fn = upd_wa_length_0"
+  and
+    \<comment>\<open>For all related Cogent and C states, the Cogent and C heaps for word arrays are related\<close>
+     srel: "\<forall>x y. (x, y) \<in> srel \<longrightarrow> (\<forall>(p :: ('a :: cogent_C_val) ptr) uv. heap_rel_meta is_v h x y p)"
+  and
+    \<comment>\<open>The type relation for word arrays\<close>
+    typrel: "type_rel (RCon ''WordArray'' [RPrim (Num num)]) TYPE('a)"
+  and
+    \<comment>\<open>The value relation for word arrays, where @{term l_c} extracts the length value and
+       @{term v_c} extracts the pointer to the array of words\<close>
+    valrelwa: "\<forall>uv (cv :: 'a). val_rel uv cv =
+      (\<exists>len arr. uv = UAbstract (UWA (TPrim (Num num)) len arr) \<and>
+      len = (SCAST(32 signed \<rightarrow> 32)(l_c cv)) \<and> arr = ptr_val (v_c cv))"
+  and
+    argn: "i < length \<gamma>"
+  and
+    valrelarg: "val_rel (\<gamma> ! i) v'"
+  and
+    argtyp: "\<Gamma>' ! i = option.Some (prod.fst (prod.snd (\<Xi>' fn)))"
+shows
+  "update_sem_init.corres wa_abs_typing_u wa_abs_repr (srel) (App (AFun fn []) (Var i))
+        (do x <- wordarray_length_c is_v h l_c (v' :: 'a ptr); gets (\<lambda>s. x) od) \<xi>0' \<gamma> \<Xi>' \<Gamma>' \<sigma> st"
+proof (rule absfun_corres[OF _ argn valrelarg])
+next 
+  show "abs_fun_rel \<Xi>' srel fn \<xi>0' (wordarray_length_c is_v h l_c) \<sigma> st (\<gamma> ! i) v'"
+    apply -
+    apply (monad_eq simp: abs_fun_rel_def wordarray_length_c_def)
+    thm imp_conjL
+    sorry    
+next
+  show "\<Gamma>' ! i = option.Some (prod.fst (prod.snd (\<Xi>' fn)))" using argtyp by assumption
+qed
+*)
 
 subsection "wordarray_get"
 
 definition wordarray_get_c
   where
   "wordarray_get_c is_v h is_vw hw l_c v_c p1_c p2_c a \<equiv>
-    do _ <- guard (\<lambda>s. is_v s (p1_c a));
-       _ <- guard (\<lambda>s. is_v s (p1_c a));
-       condition (\<lambda>s. SCAST(32 signed \<rightarrow> 32) (l_c (h s (p1_c a))) \<le> p2_c a)
-        (do ret <- gets (\<lambda>_. 0);
-            global_exn_var <- gets (\<lambda>_. Return);
-            _ <- gets (\<lambda>_. ());
-            gets (\<lambda>_. ret)
-         od)
-        (do _ <- gets (\<lambda>_. ());
-            _ <-
-            guard (\<lambda>s. is_v s (p1_c a) \<and> is_vw s (v_c (h s (p1_c a)) +\<^sub>p uint (p2_c a)));
-            _ <- guard (\<lambda>s. is_v s (p1_c a));
-            ret <-
-              do _ <- guard (\<lambda>s. is_v s (p1_c a) \<and> is_vw s (v_c (h s (p1_c a)) +\<^sub>p uint (p2_c a)));
-                 gets (\<lambda>s. hw s (v_c (h s (p1_c a)) +\<^sub>p uint (p2_c a)))
-              od;
-            global_exn_var <- gets (\<lambda>_. Return);
-            _ <- gets (\<lambda>_. ());
-            gets (\<lambda>_. ret)
-         od)
-    od"
+     do _ <- guard (\<lambda>s. is_v s (p1_c a));
+        _ <- guard (\<lambda>s. is_v s (p1_c a));
+        condition (\<lambda>s. SCAST(32 signed \<rightarrow> 32) (l_c (h s (p1_c a))) \<le> p2_c a)
+          (do ret <- gets (\<lambda>_. 0);
+              global_exn_var <- gets (\<lambda>_. Return);
+              _ <- gets (\<lambda>_. ());
+              gets (\<lambda>_. ret)
+           od)
+          (do _ <- gets (\<lambda>_. ());
+              _ <- guard (\<lambda>s. is_v s (p1_c a) \<and> is_vw s (v_c (h s (p1_c a)) +\<^sub>p uint (p2_c a)));
+              _ <- guard (\<lambda>s. is_v s (p1_c a));
+              ret <-
+                do _ <- guard (\<lambda>s. is_v s (p1_c a) \<and> is_vw s (v_c (h s (p1_c a)) +\<^sub>p uint (p2_c a)));
+                   gets (\<lambda>s. hw s (v_c (h s (p1_c a)) +\<^sub>p uint (p2_c a)))
+                od;
+              global_exn_var <- gets (\<lambda>_. Return);
+              _ <- gets (\<lambda>_. ());
+              gets (\<lambda>_. ret)
+           od)
+     od"
 
 lemma upd_C_wordarray_get_c_corres_gen:
   "\<And>i \<gamma> v' \<Gamma>' \<sigma> st.
-    \<lbrakk>\<Xi>' fn = ([], TRecord [
+    \<lbrakk>\<comment>\<open>The type of wordarray_get, where @{term fn} is name of the wordarray_get function in C,
+        @{term num} is the numeric type of the word array, @{term ptrl} is the pointer layout,
+        @{term n0}, @{term n1} are field names and these should be distinct}\<close>
+     \<Xi>' fn = ([], TRecord [
         (n0, TCon ''WordArray'' [TPrim (Num num)] (Boxed ReadOnly ptrl), Present),
         (n1, TPrim (Num U32), Present)] Unboxed, TPrim (Num num));
+     \<comment>\<open>The embedding of wordarray_get in the update semantics\<close>
      \<xi>0' fn = upd_wa_get_0;
+     \<comment>\<open>For all related Cogent and C states, the Cogent and C heaps for word arrays are related
+        and the Cogent and C heaps for the word type of the word array are related\<close>
      \<forall>x y. (x, y) \<in> srel \<longrightarrow> (\<forall>(p :: ('a :: cogent_C_val) ptr) uv. heap_rel_meta is_v h x y p) \<and>
         (\<forall>(p :: ('b :: {knows_sign,len8}) word ptr) uv. heap_rel_meta is_vw hw x y p);
+     \<comment>\<open>The type relation for word arrays\<close>
      type_rel (RCon ''WordArray'' [RPrim (Num num)]) TYPE('a);
+     \<comment>\<open>The type relation for the word type of the word arrays\<close>
      type_rel (RPrim (Num num)) TYPE('b word);
+     \<comment>\<open>The size (in bytes) of the word type of the word arrays\<close>
      size_of_num_type num = of_nat (size_of TYPE('b word));
+     \<comment>\<open>The value relation for word arrays, where @{term l_c} extracts the length value and
+        @{term v_c} extracts the pointer to the array of words\<close>
      \<forall>uv (cv :: 'a). val_rel uv cv = (\<exists>len arr. uv = UAbstract (UWA (TPrim (Num num)) len arr) \<and>
         len = (SCAST(32 signed \<rightarrow> 32)(l_c cv)) \<and> arr = ptr_val (v_c cv));
+     \<comment>\<open>The 0 values are related\<close>
      val_rel (UPrim (zero_num_lit num)) (0 :: 'b word);
+     \<comment>\<open>The value relation for the argument of wordarray_get, where @{term p1_c} extracts the first
+        field, which is a pointer to a word array, and the @{term p2_c} extracts the second field,
+        which is a 32-bit word\<close>
      \<forall>uv (cv :: 'c :: cogent_C_val). val_rel uv cv = (\<exists>p1 p2. uv = URecord [p1, p2] \<and>
         val_rel (prod.fst p1) (p1_c cv) \<and> val_rel (prod.fst p2) (p2_c cv));
+     \<comment>\<open>The rest of the assumptions are the standard value relation of arguments and what their
+        types are\<close>
      i < length \<gamma>;
      val_rel (\<gamma> ! i) v';
-     \<Gamma>' ! i = option.Some (prod.fst (prod.snd (\<Xi>' fn)))
-     \<rbrakk>
+     \<Gamma>' ! i = option.Some (prod.fst (prod.snd (\<Xi>' fn))) \<rbrakk>
     \<Longrightarrow> update_sem_init.corres wa_abs_typing_u wa_abs_repr srel (App (AFun fn []) (Var i))
          (do x <- wordarray_get_c is_v h is_vw hw l_c v_c p1_c p2_c (v' :: 'c);
              gets (\<lambda>s. x)
@@ -187,47 +248,66 @@ subsection "wordarray_put"
 definition wordarray_put_c
   where
   "wordarray_put_c is_v h is_vw hw upd_hw l_c v_c p_c i_c x_c a \<equiv>
-    do _ <- guard (\<lambda>s. is_v s (p_c a));
-       _ <-
-        do _ <- guard (\<lambda>s. is_v s (p_c a));
-          condition (\<lambda>s. i_c a < SCAST(32 signed \<rightarrow> 32) (l_c (h s (p_c a))))
-            (do _ <- guard (\<lambda>s. is_v s (p_c a) \<and> is_vw s (v_c (h s (p_c a)) +\<^sub>p uint (i_c a)));
-                _ <- guard (\<lambda>s. is_v s (p_c a));
-                _ <- guard (\<lambda>s. is_v s (p_c a) \<and> is_vw s (v_c (h s (p_c a)) +\<^sub>p uint (i_c a)));
-                modify (\<lambda>s. upd_hw (\<lambda>x. x(v_c (h s (p_c a)) +\<^sub>p uint (i_c a) := x_c a)) s)
-             od)
-            (gets (\<lambda>_. ()))
-        od;
-       ret <- gets (\<lambda>_. p_c a);
-       global_exn_var <- gets (\<lambda>_. Return);
-       _ <- gets (\<lambda>_. ());
-       gets (\<lambda>_. ret)
-    od"
+     do _ <- guard (\<lambda>s. is_v s (p_c a));
+        _ <-
+          do _ <- guard (\<lambda>s. is_v s (p_c a));
+             condition (\<lambda>s. i_c a < SCAST(32 signed \<rightarrow> 32) (l_c (h s (p_c a))))
+               (do _ <- guard (\<lambda>s. is_v s (p_c a) \<and> is_vw s (v_c (h s (p_c a)) +\<^sub>p uint (i_c a)));
+                   _ <- guard (\<lambda>s. is_v s (p_c a));
+                   _ <- guard (\<lambda>s. is_v s (p_c a) \<and> is_vw s (v_c (h s (p_c a)) +\<^sub>p uint (i_c a)));
+                   modify (\<lambda>s. upd_hw (\<lambda>x. x(v_c (h s (p_c a)) +\<^sub>p uint (i_c a) := x_c a)) s)
+                od)
+               (gets (\<lambda>_. ()))
+          od;
+        ret <- gets (\<lambda>_. p_c a);
+        global_exn_var <- gets (\<lambda>_. Return);
+        _ <- gets (\<lambda>_. ());
+        gets (\<lambda>_. ret)
+     od"
 
 lemma upd_C_wordarray_put_c_corres_gen:
   "\<And>i \<gamma> v' \<Gamma>' \<sigma> st.
-    \<lbrakk>\<Xi>' fn = ([], TRecord [
+    \<lbrakk>\<comment>\<open>The type of wordarray_put, where @{term fn} is name of the wordarray_put function in C,
+        @{term num} is the numeric type of the word array, @{term ptrl} is the pointer layout,
+        @{term n0}, @{term n1} and @{term n2} are field names and these should be distinct}\<close>
+     \<Xi>' fn = ([], TRecord [
           (n0, TCon ''WordArray'' [TPrim (Num num)] (Boxed Writable ptrl), Present),
           (n1, TPrim (Num U32), Present), (n2, TPrim (Num num), Present)] Unboxed,
         TCon ''WordArray'' [TPrim (Num num)] (Boxed Writable ptrl));
+     \<comment>\<open>The embedding of wordarray_put in the update semantics\<close>
      \<xi>0' fn = upd_wa_put2_0;
+     \<comment>\<open>For all related Cogent and C states, the Cogent and C heaps for word arrays are related
+        and the Cogent and C heaps for the word type of the word array are related\<close>
      \<forall>x y. (x, y) \<in> srel \<longrightarrow> (\<forall>(p :: ('a :: cogent_C_val) ptr) uv. heap_rel_meta is_v h x y p) \<and>
         (\<forall>(p :: ('b :: {knows_sign,len8}) word ptr) uv. heap_rel_meta is_vw hw x y p);
+     \<comment>\<open>The type relation for word arrays\<close>
      type_rel (RCon ''WordArray'' [RPrim (Num num)]) TYPE('a);
+     \<comment>\<open>The type relation for the word type of the word arrays\<close>
      type_rel (RPrim (Num num)) TYPE('b word);
+     \<comment>\<open>The size (in bytes) of the word type of the word arrays\<close>
      size_of_num_type num = of_nat (size_of TYPE('b word));
+     \<comment>\<open>The value relation for word arrays, where @{term l_c} extracts the length value and
+        @{term v_c} extracts the pointer to the array of words\<close>
      \<forall>uv (cv :: 'a). val_rel uv cv = (\<exists>len arr. uv = UAbstract (UWA (TPrim (Num num)) len arr) \<and>
         len = (SCAST(32 signed \<rightarrow> 32)(l_c cv)) \<and> arr = ptr_val (v_c cv));
+     \<comment>\<open>The value relation for the argument of wordarray_put, where @{term p_c} extracts the first
+        field, which is the pointer to a word array, @{term i_c} extracts the second field, which
+        is a 32-bit word index, and @{term x_c} extracts the third field, which is a numeric value
+        of the same type as the word array elements\<close> 
      \<forall>uv (cv :: 'c :: cogent_C_val). val_rel uv cv = (\<exists>arr i x. uv = URecord [arr, i, x] \<and>
         val_rel (prod.fst arr) (p_c cv) \<and> val_rel (prod.fst i) (i_c cv) \<and>
         val_rel (prod.fst x) ((x_c cv) :: 'b word));
+     \<comment>\<open>Assumes that updating a primitive value in the Cogent heap and the C heap should maintain
+        the state relation, where @{term upd_hw} updates the C heap mapping given a new mapping and
+        the C state. A theorem/lemma should be automatically generated to prove this assumption\<close>
      \<forall>\<sigma> st (p :: 'b word ptr) l l' v'.
         (\<sigma>, st) \<in> srel \<and> \<sigma> (ptr_val p) = option.Some (UPrim l) \<and> lit_type l = lit_type l' \<and>
         val_rel (UPrim l') v' \<longrightarrow> (\<sigma>(ptr_val p \<mapsto> UPrim l'), upd_hw (\<lambda>x. x(p := v')) st) \<in> srel;
+     \<comment>\<open>The rest of the assumptions are the standard value relation of arguments and what their
+        types are\<close>
      i < length \<gamma>;
      val_rel (\<gamma> ! i) v';
-     \<Gamma>' ! i = option.Some (prod.fst (prod.snd (\<Xi>' fn)))
-     \<rbrakk>
+     \<Gamma>' ! i = option.Some (prod.fst (prod.snd (\<Xi>' fn))) \<rbrakk>
     \<Longrightarrow> update_sem_init.corres wa_abs_typing_u wa_abs_repr srel (App (AFun fn []) (Var i))
          (do x <- wordarray_put_c is_v h is_vw hw upd_hw l_c v_c p_c i_c x_c (v' :: 'c);
              gets (\<lambda>s. x)
@@ -293,6 +373,346 @@ definition "foldmap_inv_stat obsv obsv' \<equiv> val_rel obsv obsv'"
 
 subsection "wordarray_fold_no_break"
 
+definition wordarray_fold_c
+  where
+  "wordarray_fold_c is_v h is_vw hw l_c v_c p_c s_c e_c f_c a_c o_c a_f e_upd a_upd o_upd disp a \<equiv>
+     do arg <- select UNIV;
+        _ <- guard (\<lambda>s. is_v s (p_c a));
+        ret <-
+          do _ <- guard (\<lambda>s. is_v s (p_c a));
+             condition (\<lambda>s. SCAST(32 signed \<rightarrow> 32) (l_c (h s (p_c a))) < e_c a)
+               (do _ <- guard (\<lambda>s. is_v s (p_c a));
+                   _ <- guard (\<lambda>s. is_v s (p_c a));
+                   gets (\<lambda>s. SCAST(32 signed \<rightarrow> 32) (l_c (h s (p_c a))))
+                od)
+               (gets (\<lambda>_. e_c a))
+          od;
+        e <- gets (\<lambda>_. ret);
+        arg <- gets (\<lambda>_. o_upd (\<lambda>_. o_c a) arg);
+        arg <- gets (\<lambda>_. a_upd (\<lambda>_. a_c a) arg);
+        i <- gets (\<lambda>_. s_c a);
+        (arg, i) <-
+          do _ <- guard (\<lambda>s. True);
+             whileLoop (\<lambda>(arg, i) s. i < e)
+               (\<lambda>(arg, i).
+                 do (arg, i) <-
+                    do _ <- guard (\<lambda>s. is_v s (p_c a) \<and> is_vw s (v_c (h s (p_c a)) +\<^sub>p uint i));
+                       _ <- guard (\<lambda>s. is_v s (p_c a));
+                       arg <-
+                         do _ <- guard (\<lambda>s. is_v s (p_c a) \<and> is_vw s (v_c (h s (p_c a)) +\<^sub>p uint i));
+                            gets (\<lambda>s. e_upd (\<lambda>r. hw s (v_c (h s (p_c a)) +\<^sub>p uint i)) arg)
+                         od;
+                       retval <- do ret' <- disp (f_c a) arg; gets (\<lambda>_. ret') od;
+                       arg <- gets (\<lambda>_. a_upd (\<lambda>_. retval) arg);
+                       i <- gets (\<lambda>_. i + 1);
+                       gets (\<lambda>_. (arg, i))
+                    od;
+                    _ <- guard (\<lambda>_. True);
+                    gets (\<lambda>_. (arg, i))
+                 od)
+               (arg, i)
+          od;
+        ret <- gets (\<lambda>_. a_f arg);
+        global_exn_var <- gets (\<lambda>_. Return);
+        _ <- gets (\<lambda>_. ());
+       gets (\<lambda>_. ret)
+     od"
+
+
+lemma fold_inv_step_wp:
+  "\<lbrakk>\<comment>\<open>The types of all abstract functions are well-formed\<close>
+    proc_ctx_wellformed \<Xi>';
+    \<comment>\<open>All abstract functions defined in @{term \<xi>0'} preserve typing and satisfy the frame constraints\<close>
+    upd.proc_env_matches_ptrs \<xi>0' \<Xi>';
+    \<comment>\<open>The word array value is type correct\<close>
+    wa_abs_typing_u (UWA (TPrim (Num num)) len arr) ''WordArray'' [TPrim (Num num)] (Boxed ReadOnly ptrl) r w \<sigma>;
+    \<comment>\<open>The pointer @{term p} points to the word array\<close>
+    \<sigma> p = option.Some (UAbstract (UWA (TPrim (Num num)) len arr));
+    \<comment>\<open>The accumulator value is type correct\<close>
+    upd.uval_typing \<Xi>' \<sigma> acc \<tau>a ra wa;
+    \<comment>\<open>The observer value is types correct\<close>
+    upd.uval_typing \<Xi>' \<sigma> obsv \<tau>o ro {};
+    \<comment>\<open>The accumulator writable heap footprint does not overlap with the read-only word array
+       heap footprint nor with the read-only heap footprint of the observer\<close>
+    wa \<inter> r = {}; wa \<inter> ro = {};
+    \<comment>\<open>The pointer to the word array is not in the writable heap footprint of the accumulator\<close>
+    p \<notin> wa;
+    \<comment>\<open>The type of the argument of the function , which wordarray_fold takes\<close>
+    \<tau>f = TRecord [(n0, TPrim (Num num), Present), (n1, \<tau>a, Present), (n2, \<tau>o, Present)] Unboxed;
+    \<comment>\<open>The field names are distinct\<close>
+    n0 \<noteq> n1; n0 \<noteq> n2; n1 \<noteq> n2;
+    \<comment>\<open>The function is type correct\<close>
+    (\<Xi>', [], [option.Some \<tau>f] \<turnstile> (App f (Var 0)) : \<tau>a);
+    \<comment>\<open>The function's embedding in the update semantics corresponds to its C implementation\<close>
+    \<forall>x x' \<sigma> s. val_rel x x' \<longrightarrow>
+      update_sem_init.corres wa_abs_typing_u wa_abs_repr srel
+        (App f (Var 0)) (do ret <- dispatch f_num x'; gets (\<lambda>s. ret) od)
+        \<xi>0' [x] \<Xi>' [option.Some \<tau>f] \<sigma> s;
+    \<comment>\<open>The value relation for argument to the function, where @{term elem_f} extracts the first
+       field, which contains an element from the word array, @{term acc_f} extracts the second
+       field, which is the accumulator, and @{term obsv_f} extracts the third field, which is the
+       observer\<close>
+    \<forall>uv cv. val_rel uv (cv :: 'a :: cogent_C_val) = (\<exists>elem acc obsv. uv = URecord [elem, acc, obsv] \<and>
+      val_rel (prod.fst elem) (elem_f cv) \<and> val_rel (prod.fst acc) (acc_f cv) \<and>
+      val_rel (prod.fst obsv) (obsv_f cv));
+    \<comment>\<open>Extracting the updated field returns the updated value\<close>
+    \<forall>v cv. elem_f (elem_f_upd (\<lambda>_. v) cv) = v\<rbrakk> \<Longrightarrow>
+    \<lbrace>\<lambda>sa. (a', n') = (a, n) \<and> n < e \<and>
+      (\<exists>\<sigma>' res x v. args = elem_f_upd (\<lambda>_. v) a \<and>
+        \<sigma>' (arr + size_of_num_type num * n) = option.Some x \<and> val_rel x v \<and>
+      foldmap_inv upd_wa_foldnb_bod srel \<tau>a \<tau>o \<xi>0' \<sigma> p frm n f acc obsv \<sigma>' res sa (acc_f args)) \<and>
+      foldmap_bounds frm to len n e \<and> foldmap_inv_stat obsv (obsv_f args)\<rbrace>
+      dispatch f_num args 
+    \<lbrace>\<lambda>ret sb. (\<exists>\<sigma>' res.
+        foldmap_inv upd_wa_foldnb_bod srel \<tau>a \<tau>o \<xi>0' \<sigma> p frm (n + 1) f acc obsv \<sigma>' res sb ret) \<and>
+      foldmap_inv_stat obsv (obsv_f args) \<and> foldmap_bounds frm to len (n + 1) e \<and> 
+      foldmap_measure (n + 1) to < foldmap_measure n' to\<rbrace>!"
+  apply (subst validNF_def)
+  apply clarsimp
+  apply (subst valid_def)
+  apply (subst no_fail_def)
+  apply clarsimp
+  apply (subst all_imp_conj_distrib[symmetric])
+  apply (clarsimp simp: foldmap_inv_def)
+  apply (rename_tac sa \<sigma>' res x v)
+  apply (erule_tac x = "mk_urecord [x, res, obsv]" in allE)
+  apply (erule_tac x = args in allE)
+  apply (erule impE)
+   apply (clarsimp simp: foldmap_inv_stat_def)
+  apply (erule_tac x = \<sigma>' in allE)
+  apply (erule_tac x = sa in allE)
+  apply (clarsimp simp: corres_def)
+  apply (frule_tac t = "TPrim (Num num)" and
+      ptrl = ptrl and
+      ra = r and
+      wa = w and
+      rb = ra and
+      wb = wa and
+      rc = ro in upd_wa_foldnb_bod_preservation[rotated -1];
+      simp?;
+      (clarsimp simp: Int_commute)?)
+      apply (frule wa_abs_typing_u_elims(2); clarsimp)
+     apply (frule wa_abs_typing_u_elims(2); clarsimp)
+    apply (frule wa_abs_typing_u_elims(2); clarsimp)
+   apply (frule wa_abs_typing_u_elims(2); clarsimp)
+  apply (rename_tac r' w')
+  apply (subgoal_tac "upd.matches_ptrs \<Xi>' \<sigma>' [(mk_urecord [x, res, obsv])]
+    [option.Some \<tau>f] (r' \<union> ro) w'")
+   apply clarsimp
+   apply (erule impE, blast)
+   apply clarsimp
+   apply (rename_tac ret sb)
+   apply (rotate_tac -1)
+   apply (erule_tac x = ret in allE)
+   apply (erule_tac x = sb in allE)
+   apply clarsimp
+   apply (frule upd.preservation[where \<tau>s = "[]" and K = "[]", simplified]; simp?)
+   apply clarsimp
+   apply (rename_tac \<sigma>'' res' rb wb)
+   apply (clarsimp simp: foldmap_bounds_def)
+   apply (case_tac "frm < to \<and> frm < len"; clarsimp)
+   apply (frule wa_abs_typing_u_elims(5))
+   apply (erule_tac x = n in allE; clarsimp)
+   apply (frule_tac p = "arr + (size_of_num_type num) * n" in valid_ptr_not_in_frame_same; simp?)
+    apply (drule_tac x = "arr + (size_of_num_type num) * n" and S = r in orthD1; simp?)
+    apply (drule_tac wa_abs_typing_u_elims(2)[where \<tau>s = "[_]", simplified]; simp)
+    apply blast
+   apply clarsimp
+   apply (drule_tac ta = num and 
+      arr = arr and 
+      len = len and 
+      res' = res' and 
+      \<sigma>' = \<sigma>' and 
+      \<sigma>'' = \<sigma>'' and
+      ptrl = ptrl and
+      ra = r and 
+      wa = w and
+      rc = ro in upd_wa_foldnb_bod_step[rotated -5]; simp?; clarsimp?)
+        apply (drule_tac v = obsv in upd.type_repr_uval_repr(1); simp)
+        apply (drule_tac v = res in upd.type_repr_uval_repr(1); simp)
+       apply (drule wa_abs_typing_u_elims(2); clarsimp)
+      apply (drule wa_abs_typing_u_elims(2); clarsimp)
+     apply (drule wa_abs_typing_u_elims(2); clarsimp)
+    apply (drule wa_abs_typing_u_elims(2); clarsimp)
+   apply (rule conjI)
+    apply (intro exI conjI; simp)
+   apply (frule_tac a = n and k = to in less_is_non_zero_p1)
+   apply (drule unatSuc2; clarsimp simp: word_less_nat_alt word_le_nat_alt foldmap_measure_def)
+   apply linarith
+  apply clarsimp
+  apply (rule upd.matches_ptrs_some[where r' = "{}" and w' = "{}", simplified])
+   apply (rule upd.u_t_struct; simp?)
+   apply (rule upd.u_t_r_cons1[where r = "{}" and w = "{}", simplified]; simp?)
+     apply (frule_tac wa_abs_typing_u_elims(2))
+     apply (drule_tac ?w1.0 = wa and \<sigma>' = \<sigma>' and  ?w2.0 = w' in upd.abs_typing_frame; simp?)
+     apply (drule wa_abs_typing_u_elims(5))
+     apply (erule_tac x = n in allE; clarsimp simp: foldmap_bounds_def)
+     apply (rule upd.u_t_prim'; clarsimp)
+    apply (rule upd.u_t_r_cons1[where r' = ro and w' = "{}", simplified]; simp?)
+      apply (rule upd.u_t_r_cons1[where r' = "{}" and w' = "{}", simplified]; simp?)
+        apply (drule_tac u = obsv in upd.uval_typing_frame(1); simp?)
+       apply (rule upd.u_t_r_empty)
+      apply (drule_tac v = obsv in upd.type_repr_uval_repr(1); simp)
+     apply (rule disjointI)
+     apply (rename_tac y)
+     apply (frule_tac p = y and r = ro in upd.uval_typing_valid(1)[where w = "{}", simplified]; simp?)
+     apply clarsimp
+     apply (drule_tac p = y in readonly_not_in_frame; simp?)
+     apply (drule_tac x = y and S = ro in orthD1; simp?)
+    apply (drule_tac v = res in upd.type_repr_uval_repr(1); simp)
+   apply (frule_tac wa_abs_typing_u_elims(2))
+   apply (drule_tac ?w1.0 = wa and \<sigma>' = \<sigma>' and  ?w2.0 = w' in upd.abs_typing_frame; simp?)
+   apply (drule wa_abs_typing_u_elims(5))
+   apply (erule_tac x = n in allE; clarsimp simp: foldmap_bounds_def)
+  apply (rule upd.matches_ptrs_empty[where \<tau>s = "[]", simplified])
+  done
+
+fun urecord_nth
+  where
+"urecord_nth (URecord fs) n = prod.fst (fs ! n)" |
+"urecord_nth _ _ = undefined"
+
+lemma upd_C_wordarray_fold_c_corres_gen:
+  "\<And>i \<gamma> v' \<Gamma>' \<sigma> st.
+    \<lbrakk>\<comment>\<open>The type of wordarray_fold, where @{term fn} is name of the wordarray_fold
+       function in C, @{term num} is the numeric type of the word array, @{term ptrl} is the pointer
+       layout, @{term n0}, @{term n1}, @{term n2}, @{term n3}, @{term n4} and @{term n5} are field
+       names and these should be distinct, @{term \<tau>a} is the type of the accumulator, @{term \<tau>o} is
+       the type of the observer and @{term \<tau>f} is the type of the argument to the function that
+       word_array_fold applies and the field names @{term m0}, @{term m1} and @{term m2} are distinct\<close>
+     \<Xi>' fn = ([], TRecord [
+        (n0, TCon ''WordArray'' [TPrim (Num num)] (Boxed ReadOnly ptrl), Present),
+        (n1, TPrim (Num U32), Present), (n2, TPrim (Num U32), Present), (n3, TFun \<tau>f \<tau>a, Present),
+        (n4, \<tau>a, Present), (n5, \<tau>o, Present)] Unboxed, \<tau>a);
+     \<tau>f = TRecord [(m0, TPrim (Num num), Present), (m1, \<tau>a, Present), (m2, \<tau>o, Present)] Unboxed;
+     m0 \<noteq> m1; m0 \<noteq> m2; m1 \<noteq> m2;
+     \<comment>\<open>@{term \<tau>o} is read-only i.e. has kind D or S\<close>
+     D \<in> k \<or> S \<in> k; K' \<turnstile> \<tau>o :\<kappa> k;
+     \<comment>\<open>All abstract functions defined @{term \<xi>0'} preserve typing and satisfy the frame constraints\<close>
+     upd.proc_env_matches_ptrs \<xi>0' \<Xi>';
+     \<comment>\<open>The embedding of wordarray_fold in the update semantics\<close>
+     \<xi>1' fn = upd_wa_foldnb \<Xi>' \<xi>0' \<tau>f;
+     \<comment>\<open>For all related Cogent and C states, the Cogent and C heaps for word arrays are related
+        and the Cogent and C heaps for the word type of the word array are related\<close>
+     \<forall>x y. (x, y) \<in> srel \<longrightarrow> (\<forall>(p :: ('a :: cogent_C_val) ptr) uv. heap_rel_meta is_v h x y p) \<and>
+        (\<forall>(p :: ('b :: {knows_sign,len8}) word ptr) uv. heap_rel_meta is_vw hw x y p);
+     \<comment>\<open>The type relation for word arrays\<close>
+     type_rel (RCon ''WordArray'' [RPrim (Num num)]) TYPE('a);
+     \<comment>\<open>The type relation for the word type of the word arrays\<close>
+     type_rel (RPrim (Num num)) TYPE('b word);
+     \<comment>\<open>The size (in bytes) of the word type of the word arrays\<close>
+     size_of_num_type num = of_nat (size_of TYPE('b word));
+     \<comment>\<open>The function's embedding in the update semantics corresponds to its C implementation\<close>
+     \<forall>x x' \<sigma> s. val_rel x (x' :: 'd) \<longrightarrow>
+      update_sem_init.corres wa_abs_typing_u wa_abs_repr srel
+        (App (uvalfun_to_exprfun (urecord_nth (\<gamma> ! i) 3)) (Var 0))
+        (do ret <- disp (f_c v') x'; gets (\<lambda>s. ret) od) \<xi>0' [x] \<Xi>' [option.Some \<tau>f] \<sigma> s;
+     \<comment>\<open>The function is type correct\<close>
+     \<Xi>', [], [option.Some \<tau>f] \<turnstile> App (uvalfun_to_exprfun (urecord_nth (\<gamma> ! i) 3)) (Var 0) : \<tau>a;
+     \<comment>\<open>The value relation for word arrays, where @{term l_c} extracts the length value and
+        @{term v_c} extracts the pointer to the array of words\<close>
+     \<forall>uv (cv :: 'a). val_rel uv cv = (\<exists>len arr. uv = UAbstract (UWA (TPrim (Num num)) len arr) \<and>
+        len = (SCAST(32 signed \<rightarrow> 32)(l_c cv)) \<and> arr = ptr_val (v_c cv));
+     \<comment>\<open>The value relation for the argument of wordarray_fold, where @{term p_c} extracts the pointer
+        to the word array, @{term s_c} the start index, @{term e_c} the ending index, @{term f_c}
+        the function argument, @{term a_c} the accumulator, and @{term o_c} observer\<close>
+     \<forall>uv (cv :: 'c :: cogent_C_val). val_rel uv cv = (\<exists>p s e f acc obsv.
+        uv = URecord [p, s, e, f, acc, obsv] \<and> val_rel (prod.fst p) (p_c cv) \<and>
+        val_rel (prod.fst s) (s_c cv) \<and> val_rel (prod.fst e) (e_c cv) \<and>
+        val_rel (prod.fst f) (f_c cv) \<and> val_rel (prod.fst acc) (a_c cv) \<and>
+        val_rel (prod.fst obsv) (o_c cv));
+     \<comment>\<open>The value relation for argument to the function, where @{term e_f} extracts the first
+        field, which contains an element from the word array, @{term a_f} extracts the second
+        field, which is the accumulator, and @{term o_f} extracts the third field, which is the
+        observer\<close>
+     \<forall>uv cv. val_rel uv (cv :: 'd :: cogent_C_val) = (\<exists>elem acc obsv. uv = URecord [elem, acc, obsv] \<and>
+       val_rel (prod.fst elem) (e_f cv) \<and> val_rel (prod.fst acc) (a_f cv) \<and>
+       val_rel (prod.fst obsv) (o_f cv));
+     \<comment>\<open>Extracting the updated field returns the updated value\<close>
+     \<forall>v cv. e_f (e_upd (\<lambda>_. v) cv) = v;
+     \<forall>v cv. a_f (a_upd (\<lambda>_. v) cv) = v;
+     \<forall>v cv. o_f (o_upd (\<lambda>_. v) cv) = v;
+     \<comment>\<open>Extracting field is not affected by updates to other fields\<close>
+     \<forall>v cv. e_f (a_upd (\<lambda>_. v) cv) = e_f cv;
+     \<forall>v cv. e_f (o_upd (\<lambda>_. v) cv) = e_f cv;
+     \<forall>v cv. a_f (e_upd (\<lambda>_. v) cv) = a_f cv;
+     \<forall>v cv. a_f (o_upd (\<lambda>_. v) cv) = a_f cv;
+     \<forall>v cv. o_f (e_upd (\<lambda>_. v) cv) = o_f cv;
+     \<forall>v cv. o_f (a_upd (\<lambda>_. v) cv) = o_f cv;
+     \<comment>\<open>The rest of the assumptions are the standard value relation of arguments and what their 
+        types are\<close>
+     i < length \<gamma>;
+     val_rel (\<gamma> ! i) v';
+     \<Gamma>' ! i = option.Some (prod.fst (prod.snd (\<Xi>' fn))) \<rbrakk>
+    \<Longrightarrow> update_sem_init.corres wa_abs_typing_u wa_abs_repr srel (App (AFun fn []) (Var i))
+         (do x <- wordarray_fold_c is_v h is_vw hw l_c v_c p_c s_c e_c f_c a_c o_c a_f e_upd a_upd o_upd disp (v' :: 'c);
+             gets (\<lambda>s. x)
+          od)
+         \<xi>1' \<gamma> \<Xi>' \<Gamma>' \<sigma> st"
+  apply (rule absfun_corres; simp)
+  apply (clarsimp simp: abs_fun_rel_def'; rename_tac r w)
+  apply (thin_tac "\<Gamma>' ! i = _")
+  apply (clarsimp simp: val_rel_simp)
+  apply (clarsimp simp: upd_wa_foldnb_def wordarray_fold_c_def)
+  apply (rename_tac prep frmrep torep f frep acc arep obsv orep r w warep)
+  apply (erule upd.u_t_recE; clarsimp)
+  apply (erule upd.u_t_r_consE; clarsimp)
+  apply (erule upd.u_t_p_absE; clarsimp)
+  apply (frule wa_abs_typing_u_elims(1); clarsimp)
+  apply (rename_tac r len arr)
+  apply (erule upd.u_t_r_consE; simp)
+  apply (erule upd.u_t_r_consE; simp)
+  apply (erule conjE)+
+  apply (drule_tac t = "type_repr _" in sym)+
+  apply clarsimp
+  apply (erule upd.u_t_primE)+
+  apply (drule_tac t = "lit_type _" in sym)+
+  apply clarsimp
+  apply (erule upd.u_t_r_consE; clarsimp)+
+  apply (erule upd.u_t_r_emptyE; clarsimp)
+  apply (frule upd.tfun_no_pointers(1))
+  apply (frule upd.tfun_no_pointers(2))
+  apply clarsimp
+  apply (rename_tac f acc ra wa obsv ro wo)
+  apply (drule upd.discardable_or_shareable_not_writeable; simp?)
+  apply clarsimp
+  apply (clarsimp simp: join_guards)
+  apply wp
+      apply (rename_tac var uu e)
+      apply (rule_tac M = "\<lambda>((_, i), _). foldmap_measure i (e_c v')" and 
+      I = "\<lambda>(a, b) s. (\<exists>\<sigma>' res.
+          foldmap_inv upd_wa_foldnb_bod srel \<tau>a \<tau>o \<xi>0' \<sigma> (ptr_val (p_c v'))
+          (s_c v') b (uvalfun_to_exprfun f) acc obsv \<sigma>' res s (a_f a)) \<and>
+          foldmap_inv_stat obsv (o_f a) \<and>
+          foldmap_bounds (s_c v') (e_c v') len b e" in whileLoop_add_invI; simp?)
+      apply (wp; clarsimp simp: unknown_bind_ignore split: prod.splits)
+          apply (rename_tac sa a n args a' n')
+          apply (rule_tac a = a and wa = wa and ra = ra and ro = ro and w = "{}" and r = r and
+            ptrl = ptrl and \<Xi>' = \<Xi>' and num = num  and len = len and arr = arr and ?n0.0 = m0 and
+            ?n1.0 = m1 and ?n2.0 = m2 and elem_f = e_f and acc_f = a_f and obsv_f = o_f
+            in fold_inv_step_wp; simp?) (* takes while *)
+         apply wp
+        apply wp
+       apply clarsimp
+       apply (rename_tac args j \<sigma>' res)
+       apply (clarsimp simp: foldmap_bounds_def foldmap_inv_def)
+       apply (frule wa_abs_typing_u_elims(5))
+       apply (erule_tac x = j in allE; clarsimp)
+       apply (drule_tac acc = acc and
+      obsv = obsv and
+      rb = ra and
+      wb = wa and
+      rc = ro and
+      ptrl = ptrl and
+      ra = r and
+      wa = "{}" in upd_wa_foldnb_bod_preservation; simp?; (clarsimp simp: Int_commute)?)
+  
+
+                     
+
+  
+  oops
+
 subsection "wordarray_map_no_break"
 
 section "Specialised Correspondence Theorems"
@@ -313,7 +733,8 @@ lemma upd_uprim_w32:
 subsection "wordarray_length for 32-bit word arrays"
 
 lemma wordarray_length_wordarray_length_0':
-  "wordarray_length_c is_valid_WordArray_u32_C heap_WordArray_u32_C len_C = main_pp_inferred.wordarray_length_0'"
+  "wordarray_length_c is_valid_WordArray_u32_C heap_WordArray_u32_C len_C
+    = main_pp_inferred.wordarray_length_0'"
   apply (unfold wordarray_length_c_def main_pp_inferred.wordarray_length_0'_def)
   apply (subst unknown_bind_ignore)
   apply simp
@@ -338,7 +759,8 @@ lemma upd_C_wordarray_length_u32_corres:
 subsection "wordarray_get for 32-bit word arrays"
 
 lemma wordarray_get_wordarray_get_0':
-  "wordarray_get_c is_valid_WordArray_u32_C heap_WordArray_u32_C is_valid_w32 heap_w32 len_C values_C t1_C.p1_C t1_C.p2_C = main_pp_inferred.wordarray_get_0'"
+  "wordarray_get_c is_valid_WordArray_u32_C heap_WordArray_u32_C is_valid_w32 heap_w32 len_C
+      values_C t1_C.p1_C t1_C.p2_C = main_pp_inferred.wordarray_get_0'"
   apply (unfold wordarray_get_c_def main_pp_inferred.wordarray_get_0'_def)
   apply (subst unknown_bind_ignore)
   apply simp
@@ -370,7 +792,9 @@ lemma upd_C_wordarray_get_u32_corres:
 subsection "wordarray_put2 for 32-bit word arrays"
 
 lemma wordarray_put_wordarray_put2_0':
-  "wordarray_put_c is_valid_WordArray_u32_C heap_WordArray_u32_C is_valid_w32 heap_w32 heap_w32_update len_C values_C t2_C.arr_C t2_C.idx_C t2_C.val_C  = main_pp_inferred.wordarray_put2_0'"
+  "wordarray_put_c is_valid_WordArray_u32_C heap_WordArray_u32_C is_valid_w32 heap_w32
+      heap_w32_update len_C values_C t2_C.arr_C t2_C.idx_C t2_C.val_C
+    = main_pp_inferred.wordarray_put2_0'"
   apply (unfold wordarray_put_c_def main_pp_inferred.wordarray_put2_0'_def)
   apply (subst unknown_bind_ignore)
   apply simp
@@ -401,6 +825,16 @@ lemma upd_C_wordarray_put2_u32_corres:
   done
 
 subsection "wordarray_fold_no_break for 32-bit word arrays"
+
+lemma wordarray_fold_wordarray_fold_no_break_0':
+  "wordarray_fold_c is_valid_WordArray_u32_C heap_WordArray_u32_C is_valid_w32 heap_w32 len_C
+      values_C t5_C.arr_C t5_C.frm_C t5_C.to_C t5_C.f_C t5_C.acc_C t5_C.obsv_C t3_C.acc_C
+      t3_C.elem_C_update t3_C.acc_C_update t3_C.obsv_C_update dispatch_t4'
+    = main_pp_inferred.wordarray_fold_no_break_0'"
+  apply (unfold wordarray_fold_c_def main_pp_inferred.wordarray_fold_no_break_0'_def)
+  apply (subst unknown_bind_ignore)+
+  apply simp
+  done
 end (* of context *)
 
 end
